## Question 9:

In this exercise, we prove the normalization of the Dirichlet distribution using induction. We have already shown in Exercise 2.5 that the beta distribution, which is a special case of the Dirichlet for $M = 2$, is normalized. We now assume that the Dirichlet distriution is normalized for $M - 1$ variables and prove that it is normalized for $M$ variables, and take account of the constraint $\sum_{k=1}^{M} \mu_k = 1$ by eliminating $\mu_M$, so that the Dirichlet is written:

### $$p_M (\mu_1, ..., \mu_{M-1}) = C_M \prod_{k=1}^{M-1} \mu_k^{\alpha_k - 1} \left(1 - \sum_{j=1}^{M-1} \mu_j \right)^{\alpha_M - 1}$$

and our goal is to find an expression for $C_M$. To do this, integrate over $\mu_{M-1}$, taking care over the limits of integration, and then make a change of variable so that this integral has limits 0 and 1. By assuming the correct result for $C_{M-1}$ and making use of the equation:

### $$\int_{0}^{1} \mu^{a-1} (1-\mu)^{b-1} \ d\mu = \frac{\Gamma(a) \Gamma(b)}{\Gamma(a+b)}$$

($a, b > 0$), derive the expression for $C_M$ .

---
## Solution:

We suppose that the Dirichlet distribution is normalized $\forall N \leq M - 1$ variables where $M \geq 2$ (trivial for $M = 1$ and already done in Exercise 2.5 for $M = 2$); if we have $M - 1$ variables $\\{\mu_k\\}_{i=1}^{M-1}$ that satisfy the Dirichlet conditions and Dirichlet parameters $\\{\alpha_i\\}\_{i=1}^{M-1}$, then:

### $$\int_{0}^{1} ... \int_{0}^{1} \prod_{k=1}^{M-1} \mu_k^{\alpha_k - 1} \ d\mu_{M-1} ... d\mu_1 = \dfrac{\displaystyle\prod_{i=1}^{M-1} \Gamma\left(\alpha_i\right)}{\Gamma\left(\displaystyle\sum_{i=1}^{M-1} \alpha_i\right)}$$

Now assume we have  $M$ variables $\\{\mu_k\\}_{i=1}^{M}$ that satisfy the Dirichlet condition $\displaystyle\sum\_{i=1}^{M} \mu_i = 1$ and Dirichlet parameters $\\{\alpha_i\\}\_{i=1}^{M}$, so that the distribution is given by:

### $$p_M (\mu_1, ..., \mu_{M}) = C_M \prod_{k=1}^{M} \mu_k^{\alpha_k - 1}$$

where $C_M$ is the normalization constant, so that $\displaystyle\int_{0}^{1} ... \displaystyle\int_{0}^{1} p_M (\mu_1, ..., \mu_{M}) \ d\mu_{M} ... d\mu_1 = 1$. Since $\mu_M = 1 - \displaystyle\sum_{i=1}^{M-2} \mu_i - \mu_{M-1}$, we can write:

### $$p_M (\mu_1, ..., \mu_{M-1}) = \left(C_M \prod_{k=1}^{M-2} \mu_k^{\alpha_k - 1}\right) \mu_{M-1}^{\alpha_{M-1} - 1} \left(1 - \displaystyle\sum_{j=1}^{M-1} \mu_j \right)^{\alpha_M - 1}$$

Put $t = \displaystyle\sum_{j=1}^{M-1} \mu_j$ where $\mu_j$ is fixed for all $j = 1, ..., M - 2$. So $dt = d\mu_{M-1}$ and substituting gives:

### $$1 = \int_{0}^{1} ... \int_{0}^{1} \int_{\displaystyle\sum_{j=1}^{M-2} \mu_j}^{1} \left(C_M \prod_{k=1}^{M-3} \mu_k^{\alpha_k - 1}\right) \mu_{M-2}^{\alpha_{M-2} - 1} \left(t - \displaystyle\sum_{j = 1}^{M-2} \mu_j \right)^{\alpha_{M-1} - 1} (1-t)^{\alpha_M - 1} \ dt \ d\mu_{M-2} ... d\mu_1$$

By switching the order of $t$ and $\mu_{M-2}$ (paying close attention to the limits of integration), we get:

### $$1 = \int_{0}^{1} ... \int_{0}^{1} \int_{0}^{t - \displaystyle\sum_{j=1}^{M-2} \mu_j} \left(C_M \prod_{k=1}^{M-3} \mu_k^{\alpha_k - 1}\right) \mu_{M-2}^{\alpha_{M-2} - 1} \left(t - \displaystyle\sum_{j = 1}^{M-2} \mu_j \right)^{\alpha_{M-1} - 1} (1-t)^{\alpha_M - 1} \ d\mu_{M-2} \ dt ... d\mu_1$$

Put $\mu_{M-2} = \left(t - \displaystyle\sum_{j=1}^{M-3} \mu_j \right) s$ where $s$ is the free parameter and the rest are fixed. So $d\mu_{M-2} = \left(t - \displaystyle\sum_{j=1}^{M-3} \mu_j \right) ds$ and sustituting (then simplifying) gives:

### $$1 = \int_{0}^{1} ... \int_{0}^{1} \int_{0}^{1} \left(C_M \prod_{k=1}^{M-3} \mu_k^{\alpha_k - 1}\right) \left(t - \displaystyle\sum_{j = 1}^{M-3} \mu_j \right)^{\alpha_{M-2} + \alpha_{M-1} - 1} s^{\alpha_{M-2} - 1} (1-s)^{\alpha_{M - 1} - 1} (1-t)^{\alpha_M - 1} \ ds \ dt ... d\mu_1$$

### $$1 = \left(\int_{0}^{1} ... \int_{0}^{1} \left(C_M \prod_{k=1}^{M-3} \mu_k^{\alpha_k - 1}\right) \left(t - \displaystyle\sum_{j = 1}^{M-3} \mu_j \right)^{\alpha_{M-2} + \alpha_{M-1} - 1} (1-t)^{\alpha_M - 1} \ dt ... d\mu_1 \right) \left(\int_{0}^{1} s^{\alpha_{M-2} - 1} (1-s)^{\alpha_{M - 1} - 1} \ ds \right)$$

### $$1 = \left(\int_{0}^{1} ... \int_{0}^{1} \left(C_M \prod_{k=1}^{M-3} \mu_k^{\alpha_k - 1}\right) \left(t - \displaystyle\sum_{j = 1}^{M-3} \mu_j \right)^{\alpha_{M-2} + \alpha_{M-1} - 1} (1-t)^{\alpha_M - 1} \ dt ... d\mu_1 \right) C_M \frac{\Gamma(\alpha_{M-2}) \Gamma(\alpha_{M-1})}{\Gamma(\alpha_{M-2} + \alpha_{M-1} )}$$

In the left integrand above, the expressions $\mu_k (k = 1, ..., M - 3)$, $t - \displaystyle\sum_{j=1}^{M - 3} \mu_j$ and $1-t$ sum to 1, and in total there are $M - 2$ variables. Suitable substitutions can be easily made so that the integral would take the form of a Dirichlet distribution, and thus by the inductive hypothesis we get:

### $$1 = \frac{\left(\displaystyle\prod_{i=1}^{M-3} \Gamma(\alpha_i) \right) \Gamma(\alpha_{M-2} + \alpha_{M-1}) \Gamma(\alpha_M)}{\Gamma\left(\displaystyle\sum_{i=1}^{M} \alpha_i \right)} \times C_M \frac{\Gamma(\alpha_{M-2}) \Gamma(\alpha_{M-1})}{\Gamma(\alpha_{M-2} + \alpha_{M-1} )}$$

Solving for $C_M$, we thus get:

### $$C_M = \frac{\Gamma\left(\displaystyle\sum_{i=1}^{M} \alpha_i \right)}{\displaystyle\prod_{i=1}^{M} \Gamma(\alpha_i)}$$

finishing the proof.
$$\ \ \ \ \ \ \ \ \ \ \ \ \ \ \ \ \ \ \ \ \ \ \ \ \ \ \ \ \ \ \ \ \ \ \ \ \ \ \ \ \ \ \ \ \ \ \ \ \ \ \ \ \ \ \ \ \ \ \ \ \ \ \ \ \ \ \ \ \ \ \ \ \ \ \ \ \ \ \ \ \ \ \ \ \ \ \ \ \ \ \ \ \ \ \ \ \ \ \ \ \ \ \ \ \ \ \ \ \ \ \ \ \ \ \ \ \ \ \ \ \ \ \ \ \ \ \ \ \ \ \ \ \ \ \ \ \ \ \ \ \ \ \ \ \ \ \ \ \ \ \ \ \ \ \ \ \ \ \ \ \ \ \ \ \ \ \ \ \ \ \ \ \ \ \ \ \ \ \ \ \ \ \ \ \ \ \ \ \ \ \ \ \ \ \ \ \ \ \ \ \ \ \ \ \ \ \ \ \ \ \ \ \ \ \ \ \ \ \ \ \ \ \ \ \ \ \ \ \ \ \ \ \ \ \ \ \ \ \ \ \square$$
