## Question 9:

In this exercise, we prove the normalization of the Dirichlet distribution using induction. We have already shown in Exercise 2.5 that the beta distribution, which is a special case of the Dirichlet for $M = 2$, is normalized. We now assume that the Dirichlet distriution is normalized for $M - 1$ variables and prove that it is normalized for $M$ variables, and take account of the constraint $\sum_{k=1}^{M} \mu_k = 1$ by eliminating $\mu_M$, so that the Dirichlet is written:

### $$p_M (\mu_1, ..., \mu_{M-1}) = C_M \prod_{k=1}^{M-1} \mu_k^{\alpha_k - 1} \left(1 - \sum_{j=1}^{M-1} \mu_j \right)^{\alpha_M - 1}$$

and our goal is to find an expression for $C_M$. To do this, integrate over $\mu_{M-1}$, taking care over the limits of integration, and then make a change of variable so that this integral has limits 0 and 1. By assuming the correct result for $C_{M-1}$ and making use of the equation:

### $$\int_{0}^{1} \mu^{a-1} (1-\mu)^{b-1} \ d\mu = \frac{\Gamma(a) \Gamma(b)}{\Gamma(a+b)}$$

($a, b > 0$), derive the expression for $C_M$ .

---
## Solution:

We suppose that the Dirichlet distribution is normalized for $M - 1$ variables; if we have $M - 1$ variables $\\{\mu_k\\}_{i=1}^{M-1}$ that satisfy the Dirichlet conditions and Dirichlet parameters $\\{\alpha_i\\}\_{i=1}^{M-1}$, then:

### $$\int_{0}^{\infty} ... \int_{0}^{\infty} \prod_{k=1}^{M-1} \mu_k^{\alpha_k - 1} \ d\mu_{M-1} ... d\mu_1 = \dfrac{\displaystyle\prod_{i=1}^{M-1} \Gamma\left(\alpha_i\right)}{\Gamma\left(\displaystyle\sum_{i=1}^{M-1} \alpha_i\right)}$$

Now assume we have  $M$ variables $\\{\mu_k\\}_{i=1}^{M}$ that satisfy the Dirichlet condition $\displaystyle\sum\_{i=1}^{M} \mu_i = 1$ and Dirichlet parameters $\\{\alpha_i\\}\_{i=1}^{M}$, so that the distribution is given by:

### $$p_M (\mu_1, ..., \mu_{M}) = C_M \prod_{k=1}^{M} \mu_k^{\alpha_k - 1}$$

where $C_M$ is the normalization constant, so that $\displaystyle\int_{0}^{\infty} ... \displaystyle\int_{0}^{\infty} p_M (\mu_1, ..., \mu_{M}) \ d\mu_{M} ... d\mu_1 = 1$. Since $\mu_M = 1 - \displaystyle\sum_{i=1}^{M-2} \mu_i - \mu_{M-1}$, we can write:

### $$p_M (\mu_1, ..., \mu_{M-1}) = \left(C_M \prod_{k=1}^{M-2} \mu_k^{\alpha_k - 1}\right) \mu_{M-1}^{\alpha_{M-1} - 1} \left[\left(1 - \displaystyle\sum_{j=1}^{M-2} \mu_j\right) - \mu_{M-1} \right]^{\alpha_M - 1}$$


